\section{Proof of Lemma~\ref{lem:measuresets}}\label{app:measuresets}
\begin{proof}
Let
\begin{equation}\label{eq:finiteradon}
f_N (\param) = \sum_{j=1}^{N} \frac{\eta_N (\VV^{(j)}) }{\mu (\VV^{(j)})} \Chi_{\VV^{(j)}} (\param).
\end{equation}
Then, for any $A\in\BB_\pspace$, define
\begin{equation}\label{eq:approxmeasure}
\eta (A) = \int_A f_N (\param) \, d\mu.
\end{equation}
We verify that $\eta$ is a probability measure on $(\pspace, \BB_\pspace)$ and that $\eta(A) = \eta_N(A) \; \forall \; A\in\BB_{\pspace, N}$ below:
\begin{itemize}
\item[(i)][Positive]
Let $A\in \BB_{\pspace}$.
\begin{equation*}
\begin{split}
\eta (A) &= \int_A f_N (\param) \, d\mu \\
&=  \int \Chi_A \sum_{j=1}^{N} \frac{\eta_N (\VV^{(j)}) }{\mu (\VV^{(j)})} \Chi_{\VV^{(j)}} (\param) \, d\mu \\
&= \sum_{j=1}^{N} \left ( \frac{\eta_N (\VV^{(j)}) }{\mu (\VV^{(j)})} \int \Chi_{A\cap\VV^{(j)}} (\param) \, d\mu \right ) \\
&= \sum_{j=1}^{N} \left ( \frac{\eta_N (\VV^{(j)}) }{\mu (\VV^{(j)})} \mu\left (A\cap\VV^{(j)}\right ) \right ) \geq 0
\end{split}
\end{equation*}

\item[(ii)][Definite]
\begin{equation*}
\eta (\nullset) = \int_\nullset f_N (\param) \, d\mu =\int \Chi_\nullset f_N (\param) \, d\mu = \mu(\nullset) = 0
\end{equation*}

\item[(iii)][Countably Additive]
Let $\set{A_k}_{k=1}^{\infty} \subset \BB_{\pspace}$.
\begin{equation*}
\begin{split}
\eta (\cup_k A_k) &= \int_{\cup_k A_k} f_N (\param) \, d\mu 
= \int \Chi_{\cup_k A_k} f_N (\param) \, d\mu \\
&= \int \left( \sum_k \Chi_{A_k} \right ) f_N (\param) \, d\mu
=   \sum_k \int \Chi_{A_k} f_N (\param) \, d\mu \\
&=   \sum_k \int_{A_k} f_N (\param) \, d\mu = \sum_k \eta(A_k)
\end{split}
\end{equation*}


\noindent Finally, let $A\in\BB_{\pspace, N}\subset \BB_\pspace$. 
Then there exists some $j^* \in \set{1,2, \cdots, N}$ such that $\VV^{(j^*)} = A$. 
We have that
\begin{equation*}
\begin{split}
\eta (A) &= \int_A f_N (\param) \, d\mu
=  \int \sum_{j=1}^{N} \left ( \frac{\eta_N (\VV^{(j)}) }{\mu (\VV^{(j)})} \Chi_{\VV^{(j)}}\right ) \Chi_{\VV^{(j^*)}} \, d\mu \\
&= \int \frac{\eta_N (\VV^{(j^*)}) }{\mu (\VV^{(j^*)})} \Chi_{\VV^{(j^*)}} \, d\mu
= \frac{\eta_N (\VV^{(j^*)}) }{\mu (\VV^{(j^*)})} \mu (\VV^{(j^*)}) \\
&= \eta_N (\VV^{(j^*)}) = \eta_N (A). 
\end{split}
\end{equation*}

\end{itemize}
\end{proof}


