\section{Proof of Lemma~\ref{lem:measuresets}}\label{app:measuresets}
\begin{proof}
Let
\begin{equation}
f_\nsamps (\param) = \sum_{\iparam=1}^{\nsamps} \frac{\eta_\nsamps (\VV^{(\iparam)}) }{\mu (\VV^{(\iparam)})} \Chi_{\VV^{(\iparam)}} (\param).
\end{equation}
Then, for any $A\in\BB_\pspace$, define
\begin{equation}
\eta (A) = \int_A f_\nsamps (\param) \, d\mu.
\end{equation}
We verify that $\eta$ is a probability measure on $(\pspace, \BB_\pspace)$ and that $\eta(A) = \eta_\nsamps(A) \; \forall \; A\in\BB_{\pspace, \nsamps}$ below:
\begin{itemize}
\item[(i)][Positive]
Let $A\in \BB_{\pspace}$.
\begin{equation*}
\begin{split}
\eta (A) &= \int_A f_\nsamps (\param) \, d\mu \\
&=  \int \Chi_A \sum_{\iparam=1}^{\nsamps} \frac{\eta_\nsamps (\VV^{(\iparam)}) }{\mu (\VV^{(\iparam)})} \Chi_{\VV^{(\iparam)}} (\param) \, d\mu \\
&= \sum_{\iparam=1}^{\nsamps} \left ( \frac{\eta_\nsamps (\VV^{(\iparam)}) }{\mu (\VV^{(\iparam)})} \int \Chi_{A\cap\VV^{(\iparam)}} (\param) \, d\mu \right ) \\
&= \sum_{\iparam=1}^{\nsamps} \left ( \frac{\eta_\nsamps (\VV^{(\iparam)}) }{\mu (\VV^{(\iparam)})} \mu\left (A\cap\VV^{(\iparam)}\right ) \right ) \geq 0
\end{split}
\end{equation*}

\item[(ii)][Definite]
\begin{equation*}
\eta (\nullset) = \int_\nullset f_\nsamps (\param) \, d\mu =\int \Chi_\nullset f_\nsamps (\param) \, d\mu = \mu(\nullset) = 0
\end{equation*}

\item[(iii)][Countably Additive]
Let $\set{A_k}_{k=1}^{\infty} \subset \BB_{\pspace}$.
\begin{equation*}
\begin{split}
\eta (\cup_k A_k) &= \int_{\cup_k A_k} f_\nsamps (\param) \, d\mu
= \int \Chi_{\cup_k A_k} f_\nsamps (\param) \, d\mu \\
&= \int \left( \sum_k \Chi_{A_k} \right ) f_\nsamps (\param) \, d\mu
=   \sum_k \int \Chi_{A_k} f_\nsamps (\param) \, d\mu \\
&=   \sum_k \int_{A_k} f_\nsamps (\param) \, d\mu = \sum_k \eta(A_k)
\end{split}
\end{equation*}


\noindent Finally, let $A\in\BB_{\pspace, \nsamps}\subset \BB_\pspace$.
Then there exists some $\iparam^* \in \set{1,2, \cdots, \nsamps}$ such that $\VV^{(\iparam^*)} = A$.
We have that
\begin{equation*}
\begin{split}
\eta (A) &= \int_A f_\nsamps (\param) \, d\mu
=  \int \sum_{\iparam=1}^{\nsamps} \left ( \frac{\eta_\nsamps (\VV^{(\iparam)}) }{\mu (\VV^{(\iparam)})} \Chi_{\VV^{(\iparam)}}\right ) \Chi_{\VV^{(\iparam^*)}} \, d\mu \\
&= \int \frac{\eta_\nsamps (\VV^{(\iparam^*)}) }{\mu (\VV^{(\iparam^*)})} \Chi_{\VV^{(\iparam^*)}} \, d\mu
= \frac{\eta_\nsamps (\VV^{(\iparam^*)}) }{\mu (\VV^{(\iparam^*)})} \mu (\VV^{(\iparam^*)}) \\
&= \eta_\nsamps (\VV^{(\iparam^*)}) = \eta_\nsamps (A).
\end{split}
\end{equation*}

\end{itemize}
\end{proof}
